program_logic/namespaces.v
@@ -9,7 +9,7 @@ Coercion nclose (N : namespace) : coPset := coPset_suffixes (encode N).
 
 Instance ndot_inj `{Countable A} : Inj2 (=) (=) (=) (@ndot A _ _).
 Proof. by intros N1 x1 N2 x2 ?; simplify_equality. Qed.
-Lemma nclose_nnil : nclose nnil = coPset_all.
+Lemma nclose_nnil : nclose nnil = ⊤.
 Proof. by apply (sig_eq_pi _). Qed.
 Lemma encode_nclose N : encode N ∈ nclose N.
 Proof. by apply elem_coPset_suffixes; exists xH; rewrite (left_id_L _ _). Qed.
